partialEqFull.v
@@ -4,54 +4,59 @@ Require Import partialImpliesFull.
 (*specifies that T is a source program*)
 Fixpoint initialPool T :=
   match T with
-      |Single(None,nil,e) => True
+      |Single(noTXThread id e) => True
       |_ => False
   end. 
 
 (*specifies that T has reached a terminal state*)
 Fixpoint Done T :=
   match T with
-      |Single(None,nil,v) => value v
+      |Single(noTXThread id v) => value v
       |Par T1 T2 => Done T1 /\ Done T2
       |_ => False
   end. 
 
 (*if T is done and T' is ahead of T, then T = T'*)
 Theorem DoneAheadOf : forall H T T', 
-                   Done T -> poolAheadOf H T T' ->
+                   Done T -> AheadOf H T T' ->
                    T = T'. 
 Proof.
   intros. induction H1. 
-  {inv H1. auto. inv H0. }
-  {inv H0. rewrite IHpoolAheadOf1; auto. rewrite IHpoolAheadOf2; auto. }
+  {inv H0; auto. }
+  {inv H0. }
+  {inv H0. rewrite IHAheadOf1; auto. rewrite IHAheadOf2; auto. }
 Qed. 
 
 (*the initial pool can trivially be rewound*)
-Theorem rewindInitPool : forall T C H, 
-                           initialPool T -> poolRewind C H T. 
+Theorem rewindInitPool : forall T H, 
+    initialPool T -> exists C, poolRewind C H T. 
 Proof.
-  intros. destruct T. destruct t. destruct p. destruct o. 
-  inv H0. destruct l. constructor. inv H0. inv H0. 
+  intros. destruct T.
+  {destruct t; inv H0. exists (S n). constructor. auto. }
+  {inv H0. }
 Qed. 
 
 (*If T is an initial pool, then it is trivially ahead of itself*)
-Theorem AheadOfInitPool : forall H T, initialPool T -> poolAheadOf H T T. 
+Theorem AheadOfInitPool : forall H T, initialPool T -> AheadOf H T T. 
 Proof.
-  intros. destruct T. destruct t. destruct p. destruct o. 
-  inv H0. destruct l. repeat constructor. inv H0. inv H0. 
+  intros. destruct T.
+  {destruct t; inv H0. constructor. }
+  {inv H0. }
 Qed. 
 
+
 (*partial abort and full abort are equivalent*)
-Theorem partialEqFull : forall C H T C' H' T', 
-                          initialPool T -> Done T' ->
-                          (p_multistep C H T C' H' T' <-> 
-                           f_multistep C H T C' H' T'). 
+Theorem partialEqFull : forall H T C' H' T', 
+    initialPool T -> Done T' ->
+    exists C, (p_multistep C H T C' H' T' <-> 
+          f_multistep C H T C' H' T'). 
 Proof.
-  intros. split; intros. 
-  {apply partialImpliesFullMulti. auto. apply rewindInitPool. auto. }
-  {eapply fullImpliesPartialMulti in H2. invertHyp.
-   copy H4. apply DoneAheadOf in H4; auto. subst x. eauto. apply AheadOfInitPool. 
-   auto. apply rewindInitPool. auto. }
+  intros. copy H0. apply rewindInitPool with(H := H) in H0. 
+  invertHyp. exists x. split; intros. 
+  {apply partialImpliesFullMulti; auto. }
+  {eapply fullImpliesPartialMulti in H3. invertHyp.
+   copy H5. apply DoneAheadOf in H5; auto. subst x0. eauto. auto.
+   eauto. eapply AheadOfInitPool; auto. }
 Qed. 
 
 
